More work on desugaring.

LambdaS5/coq/EjsToLjs.v
@@ -1,7 +1,10 @@
+Generalizable All Variables.
+Set Implicit Arguments.
 Require Import LjsShared.
 Require Import JsNumber.
 Require LjsSyntax.
 Require EjsSyntax.
+Require JsSyntax.
 Import ListNotations.
 Open Scope list_scope.
 Open Scope string_scope.
@@ -10,6 +13,54 @@ Local Coercion JsNumber.of_int : Z >-> JsNumber.number.
 
 Module L := LjsSyntax.
 Module E := EjsSyntax.
+Module J := JsSyntax.
+
+(* TODO move to TLC *)
+Global Instance Exists_decidable : 
+    forall `(l : list A) P (HD : forall a, Decidable (P a)), Decidable (Exists P l).
+Proof.
+    introv HD.
+    applys decidable_make (exists_st (fun a => decide (P a)) l).
+    induction l as [ | a l]; unfolds exists_st; simpl.
+    fold_bool; rew_reflect. eauto using Exists_nil_inv. 
+    rew_refl.
+    rewrite IHl.
+    remember (isTrue (P a)) as b1 eqn: Eq1.
+    destruct b1; rew_bool; fold_bool. 
+    rew_refl in *.
+    apply~ Exists_here.
+    remember (isTrue (Exists P l)) as b2 eqn: Eq2.
+    destruct b2; fold_bool.
+    rew_reflect in *.
+    apply~ Exists_next.
+    rew_reflect in *.
+    intro.
+    inverts~ H.
+Defined.
+
+(* TODO move to utilities *)
+
+Inductive Has_dupes {A : Type} : list A -> Prop :=
+    | Has_dupes_here : forall a l, Exists (fun b => a = b) l -> Has_dupes (a :: l)
+    | Has_dupes_next : forall a l, Has_dupes l -> Has_dupes (a :: l).
+
+Fixpoint has_dupes `{c : Comparable A} (l : list A) := 
+    match l with
+    | a :: l' => exists_st (fun b => decide (a = b)) l' || has_dupes l'
+    | nil => false
+    end.
+
+Global Instance Has_dupes_decidable : forall `(l : list A) `(c : Comparable A),
+    Decidable (Has_dupes l).
+Proof.
+    intros.
+    applys decidable_make (has_dupes l).
+    induction l as [ | a l]; unfold has_dupes; simpl.
+    fold_bool; rew_reflect. intro. inverts H.
+    fold has_dupes.
+    rewrite IHl.
+    skip. (* TODO *)
+Defined.
 
 Module DesugarUtils.
 
@@ -41,6 +92,8 @@ Definition to_string e :=
     | _ => make_app_builtin "%ToString" [e]
     end.
 
+Definition to_bool e := make_app_builtin "%ToBoolean" [e].
+
 Definition with_error_dispatch e :=
     L.expr_try_catch e (make_builtin "%ErrorDispatch").
 
@@ -50,17 +103,23 @@ Definition prop_accessor_check e :=
     | _ => make_app_builtin "%PropAccessorCheck" [e]
     end.
 
+(* TODO: get rid of this argsobj nonsense someday *)
 Definition make_get_field obj fld :=
     let argsobj := L.expr_object L.default_objattrs [] in
-    L.expr_get_field obj fld argsobj.
+    L.expr_get_field obj (to_string fld) argsobj.
+
+Definition make_set_field_naked obj fld v :=
+    let prop := L.property_data (L.data_intro (L.expr_id "%v") L.expr_true L.expr_true L.expr_true) in 
+    let argsobj := L.expr_object L.default_objattrs [("0", prop)] in 
+    L.expr_let "%v" v (L.expr_set_field obj (to_string fld) (L.expr_id "%v") argsobj).
 
 Definition make_set_field obj fld v :=
     match obj with
-    | L.expr_id "%context" => make_app_builtin "%EnvCheckAssign" [obj; fld; v; L.expr_id "#strict"]
-    | _ => with_error_dispatch (make_app_builtin "%set-property" [obj; fld; v])
+    | L.expr_id "%context" => make_app_builtin "%EnvCheckAssign" [obj; to_string fld; v; L.expr_id "#strict"]
+    | _ => with_error_dispatch (make_app_builtin "%set-property" [to_object obj; to_string fld; v])
     end.
 
-Definition get_while (tst bdy after : L.expr) := L.expr_undefined.
+Definition make_while (tst bdy after : L.expr) := L.expr_undefined.
 
 Definition prop_itr := 
     let tst := L.expr_op2 L.binary_op_has_own_property (L.expr_id "%obj") 
@@ -86,12 +145,122 @@ Definition make_for_in s robj bdy :=
                 (L.expr_app (L.expr_id "%get_itr") [L.expr_id "%pnameobj"])
                 (L.expr_seq
                     (make_app_builtin "%set-property" [context; sv; L.expr_app (L.expr_id "%prop_itr") []])
-                    (get_while tst bdy after))))))
+                    (make_while tst bdy after))))))
         (L.expr_if (undef_test robj) 
             L.expr_undefined
             (L.expr_if (null_test robj)
                 L.expr_undefined
                 (L.expr_app (L.expr_id "%do_loop") []))).
+
+Definition make_if e e1 e2 := L.expr_if (to_bool e) e1 e2.
+
+Definition make_throw e :=
+    L.expr_throw (L.expr_object L.default_objattrs 
+        [("%js-exn", L.property_data (L.data_intro e L.expr_false L.expr_false L.expr_false))]).
+
+Definition make_with e1 e2 := 
+    L.expr_let "%context" (make_app_builtin "%makeWithContext" [context; e1]) e2.
+
+Definition if_strict e1 e2 := L.expr_if (L.expr_id "#strict") e1 e2.
+
+Definition syntax_error s := make_app_builtin "%SyntaxError" [L.expr_string s].
+
+Definition new_context_in ctx e :=
+    L.expr_let "%parent" context (L.expr_let "%context" ctx e).
+
+Definition derived_context_in flds e :=
+    new_context_in (L.expr_object (L.objattrs_with_proto (L.expr_id "%parent") L.default_objattrs) flds) e.
+
+Definition to_js_error e := make_app_builtin "%ToJSError" [e].
+
+(*
+
+Definition create_context args body parent := 
+
+Definition make_lambda args body := 
+
+*)
+
+Definition make_fobj is (e ctx : L.expr) :=
+    ifb Exists (fun nm => nm = "arguments" \/ nm = "eval") is \/ Has_dupes is then 
+        if_strict (syntax_error "Illegal function definition") L.expr_undefined else
+    L.expr_null.
+
+Definition make_func_stmt i is e :=
+    let fobj := make_fobj is e context in
+    make_set_field_naked context (L.expr_string i) fobj.
+
+Definition make_try_catch body i catch :=
+    let prop := L.property_data (L.data_intro (to_js_error (L.expr_id i)) L.expr_true L.expr_false L.expr_false) in
+    L.expr_try_catch body (L.expr_lambda [i] (derived_context_in [(i, prop)] catch)).
+
+Definition make_xfix s e :=
+    match e with
+    | L.expr_get_field obj fld _ => make_app_builtin s [obj; fld]
+    | _ => syntax_error "Illegal use of an prefix/postfix operator"
+    end.
+
+Definition make_typeof e :=
+    match e with
+    | L.expr_get_field (L.expr_id "%context") fldexpr _ => 
+        make_app_builtin "%Typeof" [context; fldexpr]
+    | _ => L.expr_op1 L.unary_op_typeof e    
+    end.
+
+Definition make_delete e :=
+    match e with
+    | L.expr_get_field obj fldexpr _ =>
+        match obj with
+        | L.expr_id "%context" => syntax_error "Delete on context"
+        | _ => L.expr_delete_field obj (to_string fldexpr)
+        end
+    | _ => L.expr_true
+    end.
+
+Definition make_op1 op e :=
+    match op with
+    | J.unary_op_delete => make_delete e
+    | J.unary_op_post_incr => make_xfix "%PostIncrement" e
+    | J.unary_op_post_decr => make_xfix "%PostDecrement" e
+    | J.unary_op_pre_incr => make_xfix "%PrefixIncrement" e
+    | J.unary_op_pre_decr => make_xfix "%PrefixDecrement" e
+    | J.unary_op_neg => make_app_builtin "%UnaryNeg" [e]
+    | J.unary_op_add => make_app_builtin "%UnaryPlus" [e]
+    | J.unary_op_bitwise_not => make_app_builtin "%BitwiseNot" [e]
+    | J.unary_op_not => L.expr_op1 L.unary_op_not e
+    | J.unary_op_typeof => make_typeof e
+    | J.unary_op_void => L.expr_op1 L.unary_op_void e
+    end.
+
+Definition op2_func op := L.expr_lambda ["%x1";"%x2"] (L.expr_op2 op (L.expr_id "%x1") (L.expr_id "%x2")).
+
+Definition make_op2 op e1 e2 :=
+    match op with
+    | J.binary_op_coma => syntax_error "Unknown infix operator"
+    | J.binary_op_mult => make_app_builtin "%PrimMultOp" [e1; e2; op2_func L.binary_op_mul]
+    | J.binary_op_div => make_app_builtin "%PrimMultOp" [e1; e2; op2_func L.binary_op_div]
+    | J.binary_op_mod => make_app_builtin "%PrimMultOp" [e1; e2; op2_func L.binary_op_mod]
+    | J.binary_op_bitwise_and => make_app_builtin "%BitwiseInfix" [e1; e2; op2_func L.binary_op_band]
+    | J.binary_op_bitwise_or => make_app_builtin "%BitwiseInfix" [e1; e2; op2_func L.binary_op_bor]
+    | J.binary_op_bitwise_xor => make_app_builtin "%BitwiseInfix" [e1; e2; op2_func L.binary_op_bxor]
+    | J.binary_op_and => L.expr_let "%e" e1 (L.expr_if (to_bool e1) e2 (L.expr_id "%e"))
+    | J.binary_op_or => L.expr_let "%e" e1 (L.expr_if (to_bool e1) (L.expr_id "%e") e2)
+    | J.binary_op_add => make_app_builtin "%PrimAdd" [e1; e2] 
+    | J.binary_op_sub => make_app_builtin "%PrimSub" [e1; e2] 
+    | J.binary_op_left_shift => make_app_builtin "%LeftShift" [e1; e2] 
+    | J.binary_op_right_shift => make_app_builtin "%SignedRightShift" [e1; e2] 
+    | J.binary_op_unsigned_right_shift => make_app_builtin "%UnsignedRightShift" [e1; e2] 
+    | J.binary_op_lt => make_app_builtin "%LessThan" [e1; e2] 
+    | J.binary_op_gt => make_app_builtin "%GreaterThan" [e1; e2] 
+    | J.binary_op_le => make_app_builtin "%LessEqual" [e1; e2] 
+    | J.binary_op_ge => make_app_builtin "%GreaterEqual" [e1; e2] 
+    | J.binary_op_instanceof => make_app_builtin "%instanceof" [e1; e2] 
+    | J.binary_op_in => make_app_builtin "%in" [e1; e2] 
+    | J.binary_op_equal => make_app_builtin "%EqEq" [e1; e2] 
+    | J.binary_op_strict_equal => L.expr_op2 L.binary_op_stx_eq e1 e2 
+    | J.binary_op_disequal => L.expr_op1 L.unary_op_not (make_app_builtin "%EqEq" [e1; e2])
+    | J.binary_op_strict_disequal => L.expr_op1 L.unary_op_not (L.expr_op2 L.binary_op_stx_eq e1 e2)
+    end.
 
 End DesugarUtils.
 
@@ -107,25 +276,21 @@ Fixpoint ejs_to_ljs (e : E.expr) : L.expr :=
     | E.expr_string s => L.expr_string s
     | E.expr_id i => L.expr_id i
     | E.expr_this => make_builtin "%this"
+    | E.expr_func is e => make_fobj is (ejs_to_ljs e) context 
+    | E.expr_func_stmt i is e => make_func_stmt i is (ejs_to_ljs e)
     | E.expr_seq e1 e2 => L.expr_seq (ejs_to_ljs e1) (ejs_to_ljs e2)
-    | E.expr_if e e1 e2 => 
-        L.expr_if (make_app_builtin "%ToBoolean" [ejs_to_ljs e]) 
-            (ejs_to_ljs e1) (ejs_to_ljs e2)
-    | E.expr_assign e1 e2 e3 => 
-        make_set_field (to_object (ejs_to_ljs e1)) (to_string (ejs_to_ljs e2)) (ejs_to_ljs e3)
-    | E.expr_bracket e1 e2 => make_get_field (prop_accessor_check (ejs_to_ljs e1)) (to_string (ejs_to_ljs e2))
+    | E.expr_if e e1 e2 => make_if (ejs_to_ljs e) (ejs_to_ljs e1) (ejs_to_ljs e2)
+    | E.expr_op1 op e => make_op1 op (ejs_to_ljs e)
+    | E.expr_set_field e1 e2 e3 => make_set_field (ejs_to_ljs e1) (ejs_to_ljs e2) (ejs_to_ljs e3)
+    | E.expr_get_field e1 e2 => make_get_field (prop_accessor_check (ejs_to_ljs e1)) (ejs_to_ljs e2)
     | E.expr_for_in s e1 e2 => make_for_in s (ejs_to_ljs e1) (ejs_to_ljs e2) 
+    | E.expr_while e1 e2 e3 => make_while (ejs_to_ljs e1) (ejs_to_ljs e2) (ejs_to_ljs e3) 
     | E.expr_label s e => L.expr_label s (ejs_to_ljs e)
     | E.expr_break s e => L.expr_break s (ejs_to_ljs e)
-    | E.expr_throw e =>
-        L.expr_throw (L.expr_object L.default_objattrs 
-            [("%js-exn", L.property_data (L.data_intro (ejs_to_ljs e) L.expr_false L.expr_false L.expr_false))])
-    | E.expr_try_finally e1 e2 =>  
-        L.expr_try_finally (ejs_to_ljs e1) (ejs_to_ljs e2)
-    | E.expr_with e1 e2 =>
-        L.expr_let "%context" 
-            (make_app_builtin "%makeWithContext" [context; ejs_to_ljs e1]) 
-            (ejs_to_ljs e2)
+    | E.expr_throw e => make_throw (ejs_to_ljs e)
+    | E.expr_try_catch e1 i e2 => make_try_catch (ejs_to_ljs e1) i (ejs_to_ljs e2)
+    | E.expr_try_finally e1 e2 => L.expr_try_finally (ejs_to_ljs e1) (ejs_to_ljs e2)
+    | E.expr_with e1 e2 => make_with (ejs_to_ljs e1) (ejs_to_ljs e2)
     | E.expr_strict e => L.expr_let "#strict" L.expr_true (ejs_to_ljs e)
     | E.expr_nonstrict e => L.expr_let "#strict" L.expr_false (ejs_to_ljs e)
     | _ => L.expr_dump
