LambdaS5/coq/LjsSyntax.v
@@ -146,6 +146,8 @@ with objattrs : Type :=
 
 Definition default_objattrs := objattrs_intro (expr_string "Object") expr_true expr_null expr_null expr_undefined.
 
+Definition objattrs_with_proto p oa := let 'objattrs_intro cl ex pr co pv := oa in objattrs_intro cl ex p co pv.
+
 (* Lexical environments *)
 
 Definition loc_heap_type := Heap.heap id value_loc.
